Porting to VST 2.3alpha, round1

dig/digest.v
@@ -1,94 +1,109 @@
-
-Require Import Clightdefs.
+From Coq Require Import String List ZArith.
+From compcert Require Import Coqlib Integers Floats AST Ctypes Cop Clight Clightdefs.
 Local Open Scope Z_scope.
-Definition _ERR_put_error : ident := 72%positive.
-Definition _EVP_Digest : ident := 113%positive.
-Definition _EVP_DigestFinal : ident := 107%positive.
-Definition _EVP_DigestFinal_ex : ident := 106%positive.
-Definition _EVP_DigestInit : ident := 100%positive.
-Definition _EVP_DigestInit_ex : ident := 99%positive.
-Definition _EVP_DigestUpdate : ident := 103%positive.
-Definition _EVP_MD_CTX_block_size : ident := 116%positive.
-Definition _EVP_MD_CTX_cleanup : ident := 89%positive.
-Definition _EVP_MD_CTX_copy : ident := 96%positive.
-Definition _EVP_MD_CTX_copy_ex : ident := 95%positive.
-Definition _EVP_MD_CTX_create : ident := 88%positive.
-Definition _EVP_MD_CTX_destroy : ident := 90%positive.
-Definition _EVP_MD_CTX_init : ident := 87%positive.
-Definition _EVP_MD_CTX_md : ident := 114%positive.
-Definition _EVP_MD_CTX_size : ident := 115%positive.
-Definition _EVP_MD_CTX_type : ident := 117%positive.
-Definition _EVP_MD_block_size : ident := 85%positive.
-Definition _EVP_MD_flags : ident := 83%positive.
-Definition _EVP_MD_size : ident := 84%positive.
-Definition _EVP_MD_type : ident := 82%positive.
-Definition _EVP_add_digest : ident := 118%positive.
-Definition _OPENSSL_cleanse : ident := 74%positive.
-Definition _OPENSSL_memcpy : ident := 78%positive.
-Definition _OPENSSL_memset : ident := 80%positive.
-Definition ___builtin_annot : ident := 21%positive.
-Definition ___builtin_annot_intval : ident := 22%positive.
-Definition ___builtin_bswap : ident := 47%positive.
-Definition ___builtin_bswap16 : ident := 50%positive.
-Definition ___builtin_bswap32 : ident := 49%positive.
-Definition ___builtin_bswap64 : ident := 48%positive.
-Definition ___builtin_clz : ident := 51%positive.
-Definition ___builtin_clzl : ident := 52%positive.
-Definition ___builtin_clzll : ident := 53%positive.
-Definition ___builtin_ctz : ident := 54%positive.
-Definition ___builtin_ctzl : ident := 55%positive.
-Definition ___builtin_ctzll : ident := 56%positive.
-Definition ___builtin_debug : ident := 69%positive.
-Definition ___builtin_fabs : ident := 19%positive.
-Definition ___builtin_fmadd : ident := 60%positive.
-Definition ___builtin_fmax : ident := 58%positive.
-Definition ___builtin_fmin : ident := 59%positive.
-Definition ___builtin_fmsub : ident := 61%positive.
-Definition ___builtin_fnmadd : ident := 62%positive.
-Definition ___builtin_fnmsub : ident := 63%positive.
-Definition ___builtin_fsqrt : ident := 57%positive.
-Definition ___builtin_membar : ident := 23%positive.
-Definition ___builtin_memcpy_aligned : ident := 20%positive.
-Definition ___builtin_nop : ident := 68%positive.
-Definition ___builtin_read16_reversed : ident := 64%positive.
-Definition ___builtin_read32_reversed : ident := 65%positive.
-Definition ___builtin_va_arg : ident := 25%positive.
-Definition ___builtin_va_copy : ident := 26%positive.
-Definition ___builtin_va_end : ident := 27%positive.
-Definition ___builtin_va_start : ident := 24%positive.
-Definition ___builtin_write16_reversed : ident := 66%positive.
-Definition ___builtin_write32_reversed : ident := 67%positive.
-Definition ___compcert_va_composite : ident := 31%positive.
-Definition ___compcert_va_float64 : ident := 30%positive.
-Definition ___compcert_va_int32 : ident := 28%positive.
-Definition ___compcert_va_int64 : ident := 29%positive.
-Definition ___i64_dtos : ident := 32%positive.
-Definition ___i64_dtou : ident := 33%positive.
-Definition ___i64_sar : ident := 44%positive.
-Definition ___i64_sdiv : ident := 38%positive.
-Definition ___i64_shl : ident := 42%positive.
-Definition ___i64_shr : ident := 43%positive.
-Definition ___i64_smod : ident := 40%positive.
-Definition ___i64_smulh : ident := 45%positive.
-Definition ___i64_stod : ident := 34%positive.
-Definition ___i64_stof : ident := 36%positive.
-Definition ___i64_udiv : ident := 39%positive.
-Definition ___i64_umod : ident := 41%positive.
-Definition ___i64_umulh : ident := 46%positive.
-Definition ___i64_utod : ident := 35%positive.
-Definition ___i64_utof : ident := 37%positive.
-Definition ___stringlit_1 : ident := 94%positive.
+
+Module Info.
+  Definition version := "3.4"%string.
+  Definition build_number := ""%string.
+  Definition build_tag := ""%string.
+  Definition arch := "x86"%string.
+  Definition model := "32sse2"%string.
+  Definition abi := "standard"%string.
+  Definition bitsize := 32.
+  Definition big_endian := false.
+  Definition source_file := "digest.c"%string.
+  Definition normalized := true.
+End Info.
+
+Definition _ERR_put_error : ident := 73%positive.
+Definition _EVP_Digest : ident := 114%positive.
+Definition _EVP_DigestFinal : ident := 108%positive.
+Definition _EVP_DigestFinal_ex : ident := 107%positive.
+Definition _EVP_DigestInit : ident := 101%positive.
+Definition _EVP_DigestInit_ex : ident := 100%positive.
+Definition _EVP_DigestUpdate : ident := 104%positive.
+Definition _EVP_MD_CTX_block_size : ident := 117%positive.
+Definition _EVP_MD_CTX_cleanup : ident := 90%positive.
+Definition _EVP_MD_CTX_copy : ident := 97%positive.
+Definition _EVP_MD_CTX_copy_ex : ident := 96%positive.
+Definition _EVP_MD_CTX_create : ident := 89%positive.
+Definition _EVP_MD_CTX_destroy : ident := 91%positive.
+Definition _EVP_MD_CTX_init : ident := 88%positive.
+Definition _EVP_MD_CTX_md : ident := 115%positive.
+Definition _EVP_MD_CTX_size : ident := 116%positive.
+Definition _EVP_MD_CTX_type : ident := 118%positive.
+Definition _EVP_MD_block_size : ident := 86%positive.
+Definition _EVP_MD_flags : ident := 84%positive.
+Definition _EVP_MD_size : ident := 85%positive.
+Definition _EVP_MD_type : ident := 83%positive.
+Definition _EVP_add_digest : ident := 119%positive.
+Definition _OPENSSL_cleanse : ident := 75%positive.
+Definition _OPENSSL_memcpy : ident := 79%positive.
+Definition _OPENSSL_memset : ident := 81%positive.
+Definition ___builtin_ais_annot : ident := 19%positive.
+Definition ___builtin_annot : ident := 26%positive.
+Definition ___builtin_annot_intval : ident := 27%positive.
+Definition ___builtin_bswap : ident := 20%positive.
+Definition ___builtin_bswap16 : ident := 22%positive.
+Definition ___builtin_bswap32 : ident := 21%positive.
+Definition ___builtin_bswap64 : ident := 52%positive.
+Definition ___builtin_clz : ident := 53%positive.
+Definition ___builtin_clzl : ident := 54%positive.
+Definition ___builtin_clzll : ident := 55%positive.
+Definition ___builtin_ctz : ident := 56%positive.
+Definition ___builtin_ctzl : ident := 57%positive.
+Definition ___builtin_ctzll : ident := 58%positive.
+Definition ___builtin_debug : ident := 70%positive.
+Definition ___builtin_fabs : ident := 23%positive.
+Definition ___builtin_fmadd : ident := 61%positive.
+Definition ___builtin_fmax : ident := 59%positive.
+Definition ___builtin_fmin : ident := 60%positive.
+Definition ___builtin_fmsub : ident := 62%positive.
+Definition ___builtin_fnmadd : ident := 63%positive.
+Definition ___builtin_fnmsub : ident := 64%positive.
+Definition ___builtin_fsqrt : ident := 24%positive.
+Definition ___builtin_membar : ident := 28%positive.
+Definition ___builtin_memcpy_aligned : ident := 25%positive.
+Definition ___builtin_nop : ident := 69%positive.
+Definition ___builtin_read16_reversed : ident := 65%positive.
+Definition ___builtin_read32_reversed : ident := 66%positive.
+Definition ___builtin_va_arg : ident := 30%positive.
+Definition ___builtin_va_copy : ident := 31%positive.
+Definition ___builtin_va_end : ident := 32%positive.
+Definition ___builtin_va_start : ident := 29%positive.
+Definition ___builtin_write16_reversed : ident := 67%positive.
+Definition ___builtin_write32_reversed : ident := 68%positive.
+Definition ___compcert_i64_dtos : ident := 37%positive.
+Definition ___compcert_i64_dtou : ident := 38%positive.
+Definition ___compcert_i64_sar : ident := 49%positive.
+Definition ___compcert_i64_sdiv : ident := 43%positive.
+Definition ___compcert_i64_shl : ident := 47%positive.
+Definition ___compcert_i64_shr : ident := 48%positive.
+Definition ___compcert_i64_smod : ident := 45%positive.
+Definition ___compcert_i64_smulh : ident := 50%positive.
+Definition ___compcert_i64_stod : ident := 39%positive.
+Definition ___compcert_i64_stof : ident := 41%positive.
+Definition ___compcert_i64_udiv : ident := 44%positive.
+Definition ___compcert_i64_umod : ident := 46%positive.
+Definition ___compcert_i64_umulh : ident := 51%positive.
+Definition ___compcert_i64_utod : ident := 40%positive.
+Definition ___compcert_i64_utof : ident := 42%positive.
+Definition ___compcert_va_composite : ident := 36%positive.
+Definition ___compcert_va_float64 : ident := 35%positive.
+Definition ___compcert_va_int32 : ident := 33%positive.
+Definition ___compcert_va_int64 : ident := 34%positive.
+Definition ___stringlit_1 : ident := 95%positive.
 Definition _block_size : ident := 15%positive.
-Definition _c : ident := 79%positive.
-Definition _count : ident := 108%positive.
-Definition _ctx : ident := 86%positive.
+Definition _c : ident := 80%positive.
+Definition _count : ident := 109%positive.
+Definition _ctx : ident := 87%positive.
 Definition _ctx_size : ident := 16%positive.
-Definition _data : ident := 101%positive.
+Definition _data : ident := 102%positive.
 Definition _digest : ident := 2%positive.
-Definition _dst : ident := 75%positive.
+Definition _dst : ident := 76%positive.
 Definition _dup : ident := 18%positive.
-Definition _engine : ident := 97%positive.
-Definition _engine_st : ident := 98%positive.
+Definition _engine : ident := 98%positive.
+Definition _engine_st : ident := 99%positive.
 Definition _env_md_ctx_st : ident := 8%positive.
 Definition _env_md_st : ident := 1%positive.
 Definition _evp_md_pctx_ops : ident := 6%positive.
@@ -96,56 +111,56 @@ Definition _evp_pkey_ctx_st : ident := 4%positive.
 Definition _final : ident := 14%positive.
 Definition _flags : ident := 11%positive.
 Definition _free : ident := 17%positive.
-Definition _impl : ident := 111%positive.
-Definition _in : ident := 92%positive.
+Definition _impl : ident := 112%positive.
+Definition _in : ident := 93%positive.
 Definition _init : ident := 12%positive.
-Definition _len : ident := 102%positive.
-Definition _main : ident := 119%positive.
-Definition _malloc : ident := 73%positive.
-Definition _md : ident := 81%positive.
+Definition _len : ident := 103%positive.
+Definition _main : ident := 120%positive.
+Definition _malloc : ident := 74%positive.
+Definition _md : ident := 82%positive.
 Definition _md_data : ident := 3%positive.
-Definition _md_out : ident := 104%positive.
+Definition _md_out : ident := 105%positive.
 Definition _md_size : ident := 10%positive.
-Definition _memcpy : ident := 70%positive.
-Definition _memset : ident := 71%positive.
-Definition _n : ident := 77%positive.
-Definition _out : ident := 91%positive.
-Definition _out_md : ident := 109%positive.
-Definition _out_size : ident := 110%positive.
+Definition _memcpy : ident := 71%positive.
+Definition _memset : ident := 72%positive.
+Definition _n : ident := 78%positive.
+Definition _out : ident := 92%positive.
+Definition _out_md : ident := 110%positive.
+Definition _out_size : ident := 111%positive.
 Definition _pctx : ident := 5%positive.
 Definition _pctx_ops : ident := 7%positive.
-Definition _ret : ident := 112%positive.
-Definition _size : ident := 105%positive.
-Definition _src : ident := 76%positive.
-Definition _tmp_buf : ident := 93%positive.
+Definition _ret : ident := 113%positive.
+Definition _size : ident := 106%positive.
+Definition _src : ident := 77%positive.
+Definition _tmp_buf : ident := 94%positive.
 Definition _type : ident := 9%positive.
 Definition _update : ident := 13%positive.
-Definition _t'1 : ident := 120%positive.
-Definition _t'10 : ident := 129%positive.
-Definition _t'11 : ident := 130%positive.
-Definition _t'12 : ident := 131%positive.
-Definition _t'13 : ident := 132%positive.
-Definition _t'14 : ident := 133%positive.
-Definition _t'15 : ident := 134%positive.
-Definition _t'16 : ident := 135%positive.
-Definition _t'17 : ident := 136%positive.
-Definition _t'18 : ident := 137%positive.
-Definition _t'19 : ident := 138%positive.
-Definition _t'2 : ident := 121%positive.
-Definition _t'20 : ident := 139%positive.
-Definition _t'21 : ident := 140%positive.
-Definition _t'22 : ident := 141%positive.
-Definition _t'23 : ident := 142%positive.
-Definition _t'24 : ident := 143%positive.
-Definition _t'25 : ident := 144%positive.
-Definition _t'26 : ident := 145%positive.
-Definition _t'3 : ident := 122%positive.
-Definition _t'4 : ident := 123%positive.
-Definition _t'5 : ident := 124%positive.
-Definition _t'6 : ident := 125%positive.
-Definition _t'7 : ident := 126%positive.
-Definition _t'8 : ident := 127%positive.
-Definition _t'9 : ident := 128%positive.
+Definition _t'1 : ident := 121%positive.
+Definition _t'10 : ident := 130%positive.
+Definition _t'11 : ident := 131%positive.
+Definition _t'12 : ident := 132%positive.
+Definition _t'13 : ident := 133%positive.
+Definition _t'14 : ident := 134%positive.
+Definition _t'15 : ident := 135%positive.
+Definition _t'16 : ident := 136%positive.
+Definition _t'17 : ident := 137%positive.
+Definition _t'18 : ident := 138%positive.
+Definition _t'19 : ident := 139%positive.
+Definition _t'2 : ident := 122%positive.
+Definition _t'20 : ident := 140%positive.
+Definition _t'21 : ident := 141%positive.
+Definition _t'22 : ident := 142%positive.
+Definition _t'23 : ident := 143%positive.
+Definition _t'24 : ident := 144%positive.
+Definition _t'25 : ident := 145%positive.
+Definition _t'26 : ident := 146%positive.
+Definition _t'3 : ident := 123%positive.
+Definition _t'4 : ident := 124%positive.
+Definition _t'5 : ident := 125%positive.
+Definition _t'6 : ident := 126%positive.
+Definition _t'7 : ident := 127%positive.
+Definition _t'8 : ident := 128%positive.
+Definition _t'9 : ident := 129%positive.
 
 Definition v___stringlit_1 := {|
   gvar_info := (tarray tschar 9);
@@ -1390,10 +1405,32 @@ Definition composites : list composite_definition :=
              (tptr (Tstruct _evp_pkey_ctx_st noattr)) cc_default))) :: nil)
    noattr :: nil).
 
-Definition global_definitions :=
+Definition global_definitions : list (ident * globdef fundef type) :=
 ((___stringlit_1, Gvar v___stringlit_1) ::
+ (___builtin_ais_annot,
+   Gfun(External (EF_builtin "__builtin_ais_annot"
+                   (mksignature (AST.Tint :: nil) None
+                     {|cc_vararg:=true; cc_unproto:=false; cc_structret:=false|}))
+     (Tcons (tptr tschar) Tnil) tvoid
+     {|cc_vararg:=true; cc_unproto:=false; cc_structret:=false|})) ::
+ (___builtin_bswap,
+   Gfun(External (EF_builtin "__builtin_bswap"
+                   (mksignature (AST.Tint :: nil) (Some AST.Tint) cc_default))
+     (Tcons tuint Tnil) tuint cc_default)) ::
+ (___builtin_bswap32,
+   Gfun(External (EF_builtin "__builtin_bswap32"
+                   (mksignature (AST.Tint :: nil) (Some AST.Tint) cc_default))
+     (Tcons tuint Tnil) tuint cc_default)) ::
+ (___builtin_bswap16,
+   Gfun(External (EF_builtin "__builtin_bswap16"
+                   (mksignature (AST.Tint :: nil) (Some AST.Tint) cc_default))
+     (Tcons tushort Tnil) tushort cc_default)) ::
  (___builtin_fabs,
    Gfun(External (EF_builtin "__builtin_fabs"
+                   (mksignature (AST.Tfloat :: nil) (Some AST.Tfloat)
+                     cc_default)) (Tcons tdouble Tnil) tdouble cc_default)) ::
+ (___builtin_fsqrt,
+   Gfun(External (EF_builtin "__builtin_fsqrt"
                    (mksignature (AST.Tfloat :: nil) (Some AST.Tfloat)
                      cc_default)) (Tcons tdouble Tnil) tdouble cc_default)) ::
  (___builtin_memcpy_aligned,
@@ -1455,91 +1492,79 @@ Definition global_definitions :=
                    (mksignature (AST.Tint :: AST.Tint :: nil) (Some AST.Tint)
                      cc_default)) (Tcons (tptr tvoid) (Tcons tuint Tnil))
      (tptr tvoid) cc_default)) ::
- (___i64_dtos,
-   Gfun(External (EF_runtime "__i64_dtos"
+ (___compcert_i64_dtos,
+   Gfun(External (EF_runtime "__compcert_i64_dtos"
                    (mksignature (AST.Tfloat :: nil) (Some AST.Tlong)
                      cc_default)) (Tcons tdouble Tnil) tlong cc_default)) ::
- (___i64_dtou,
-   Gfun(External (EF_runtime "__i64_dtou"
+ (___compcert_i64_dtou,
+   Gfun(External (EF_runtime "__compcert_i64_dtou"
                    (mksignature (AST.Tfloat :: nil) (Some AST.Tlong)
                      cc_default)) (Tcons tdouble Tnil) tulong cc_default)) ::
- (___i64_stod,
-   Gfun(External (EF_runtime "__i64_stod"
+ (___compcert_i64_stod,
+   Gfun(External (EF_runtime "__compcert_i64_stod"
                    (mksignature (AST.Tlong :: nil) (Some AST.Tfloat)
                      cc_default)) (Tcons tlong Tnil) tdouble cc_default)) ::
- (___i64_utod,
-   Gfun(External (EF_runtime "__i64_utod"
+ (___compcert_i64_utod,
+   Gfun(External (EF_runtime "__compcert_i64_utod"
                    (mksignature (AST.Tlong :: nil) (Some AST.Tfloat)
                      cc_default)) (Tcons tulong Tnil) tdouble cc_default)) ::
- (___i64_stof,
-   Gfun(External (EF_runtime "__i64_stof"
+ (___compcert_i64_stof,
+   Gfun(External (EF_runtime "__compcert_i64_stof"
                    (mksignature (AST.Tlong :: nil) (Some AST.Tsingle)
                      cc_default)) (Tcons tlong Tnil) tfloat cc_default)) ::
- (___i64_utof,
-   Gfun(External (EF_runtime "__i64_utof"
+ (___compcert_i64_utof,
+   Gfun(External (EF_runtime "__compcert_i64_utof"
                    (mksignature (AST.Tlong :: nil) (Some AST.Tsingle)
                      cc_default)) (Tcons tulong Tnil) tfloat cc_default)) ::
- (___i64_sdiv,
-   Gfun(External (EF_runtime "__i64_sdiv"
+ (___compcert_i64_sdiv,
+   Gfun(External (EF_runtime "__compcert_i64_sdiv"
                    (mksignature (AST.Tlong :: AST.Tlong :: nil)
                      (Some AST.Tlong) cc_default))
      (Tcons tlong (Tcons tlong Tnil)) tlong cc_default)) ::
- (___i64_udiv,
-   Gfun(External (EF_runtime "__i64_udiv"
+ (___compcert_i64_udiv,
+   Gfun(External (EF_runtime "__compcert_i64_udiv"
                    (mksignature (AST.Tlong :: AST.Tlong :: nil)
                      (Some AST.Tlong) cc_default))
      (Tcons tulong (Tcons tulong Tnil)) tulong cc_default)) ::
- (___i64_smod,
-   Gfun(External (EF_runtime "__i64_smod"
+ (___compcert_i64_smod,
+   Gfun(External (EF_runtime "__compcert_i64_smod"
                    (mksignature (AST.Tlong :: AST.Tlong :: nil)
                      (Some AST.Tlong) cc_default))
      (Tcons tlong (Tcons tlong Tnil)) tlong cc_default)) ::
- (___i64_umod,
-   Gfun(External (EF_runtime "__i64_umod"
+ (___compcert_i64_umod,
+   Gfun(External (EF_runtime "__compcert_i64_umod"
                    (mksignature (AST.Tlong :: AST.Tlong :: nil)
                      (Some AST.Tlong) cc_default))
      (Tcons tulong (Tcons tulong Tnil)) tulong cc_default)) ::
- (___i64_shl,
-   Gfun(External (EF_runtime "__i64_shl"
+ (___compcert_i64_shl,
+   Gfun(External (EF_runtime "__compcert_i64_shl"
                    (mksignature (AST.Tlong :: AST.Tint :: nil)
                      (Some AST.Tlong) cc_default))
      (Tcons tlong (Tcons tint Tnil)) tlong cc_default)) ::
- (___i64_shr,
-   Gfun(External (EF_runtime "__i64_shr"
+ (___compcert_i64_shr,
+   Gfun(External (EF_runtime "__compcert_i64_shr"
                    (mksignature (AST.Tlong :: AST.Tint :: nil)
                      (Some AST.Tlong) cc_default))
      (Tcons tulong (Tcons tint Tnil)) tulong cc_default)) ::
- (___i64_sar,
-   Gfun(External (EF_runtime "__i64_sar"
+ (___compcert_i64_sar,
+   Gfun(External (EF_runtime "__compcert_i64_sar"
                    (mksignature (AST.Tlong :: AST.Tint :: nil)
                      (Some AST.Tlong) cc_default))
      (Tcons tlong (Tcons tint Tnil)) tlong cc_default)) ::
- (___i64_smulh,
-   Gfun(External (EF_runtime "__i64_smulh"
+ (___compcert_i64_smulh,
+   Gfun(External (EF_runtime "__compcert_i64_smulh"
                    (mksignature (AST.Tlong :: AST.Tlong :: nil)
                      (Some AST.Tlong) cc_default))
      (Tcons tlong (Tcons tlong Tnil)) tlong cc_default)) ::
- (___i64_umulh,
-   Gfun(External (EF_runtime "__i64_umulh"
+ (___compcert_i64_umulh,
+   Gfun(External (EF_runtime "__compcert_i64_umulh"
                    (mksignature (AST.Tlong :: AST.Tlong :: nil)
                      (Some AST.Tlong) cc_default))
      (Tcons tulong (Tcons tulong Tnil)) tulong cc_default)) ::
- (___builtin_bswap,
-   Gfun(External (EF_builtin "__builtin_bswap"
-                   (mksignature (AST.Tint :: nil) (Some AST.Tint) cc_default))
-     (Tcons tuint Tnil) tuint cc_default)) ::
  (___builtin_bswap64,
    Gfun(External (EF_builtin "__builtin_bswap64"
                    (mksignature (AST.Tlong :: nil) (Some AST.Tlong)
                      cc_default)) (Tcons tulong Tnil) tulong cc_default)) ::
- (___builtin_bswap32,
-   Gfun(External (EF_builtin "__builtin_bswap32"
-                   (mksignature (AST.Tint :: nil) (Some AST.Tint) cc_default))
-     (Tcons tuint Tnil) tuint cc_default)) ::
- (___builtin_bswap16,
-   Gfun(External (EF_builtin "__builtin_bswap16"
-                   (mksignature (AST.Tint :: nil) (Some AST.Tint) cc_default))
-     (Tcons tushort Tnil) tushort cc_default)) ::
  (___builtin_clz,
    Gfun(External (EF_builtin "__builtin_clz"
                    (mksignature (AST.Tint :: nil) (Some AST.Tint) cc_default))
@@ -1564,10 +1589,6 @@ Definition global_definitions :=
    Gfun(External (EF_builtin "__builtin_ctzll"
                    (mksignature (AST.Tlong :: nil) (Some AST.Tint)
                      cc_default)) (Tcons tulong Tnil) tint cc_default)) ::
- (___builtin_fsqrt,
-   Gfun(External (EF_builtin "__builtin_fsqrt"
-                   (mksignature (AST.Tfloat :: nil) (Some AST.Tfloat)
-                     cc_default)) (Tcons tdouble Tnil) tdouble cc_default)) ::
  (___builtin_fmax,
    Gfun(External (EF_builtin "__builtin_fmax"
                    (mksignature (AST.Tfloat :: AST.Tfloat :: nil)
@@ -1685,7 +1706,7 @@ Definition global_definitions :=
  (_EVP_MD_CTX_type, Gfun(Internal f_EVP_MD_CTX_type)) ::
  (_EVP_add_digest, Gfun(Internal f_EVP_add_digest)) :: nil).
 
-Definition public_idents :=
+Definition public_idents : list ident :=
 (_EVP_add_digest :: _EVP_MD_CTX_type :: _EVP_MD_CTX_block_size ::
  _EVP_MD_CTX_size :: _EVP_MD_CTX_md :: _EVP_Digest :: _EVP_DigestFinal ::
  _EVP_DigestFinal_ex :: _EVP_DigestUpdate :: _EVP_DigestInit ::
@@ -1698,17 +1719,20 @@ Definition public_idents :=
  ___builtin_read32_reversed :: ___builtin_read16_reversed ::
  ___builtin_fnmsub :: ___builtin_fnmadd :: ___builtin_fmsub ::
  ___builtin_fmadd :: ___builtin_fmin :: ___builtin_fmax ::
- ___builtin_fsqrt :: ___builtin_ctzll :: ___builtin_ctzl :: ___builtin_ctz ::
- ___builtin_clzll :: ___builtin_clzl :: ___builtin_clz ::
- ___builtin_bswap16 :: ___builtin_bswap32 :: ___builtin_bswap64 ::
- ___builtin_bswap :: ___i64_umulh :: ___i64_smulh :: ___i64_sar ::
- ___i64_shr :: ___i64_shl :: ___i64_umod :: ___i64_smod :: ___i64_udiv ::
- ___i64_sdiv :: ___i64_utof :: ___i64_stof :: ___i64_utod :: ___i64_stod ::
- ___i64_dtou :: ___i64_dtos :: ___compcert_va_composite ::
- ___compcert_va_float64 :: ___compcert_va_int64 :: ___compcert_va_int32 ::
- ___builtin_va_end :: ___builtin_va_copy :: ___builtin_va_arg ::
- ___builtin_va_start :: ___builtin_membar :: ___builtin_annot_intval ::
- ___builtin_annot :: ___builtin_memcpy_aligned :: ___builtin_fabs :: nil).
+ ___builtin_ctzll :: ___builtin_ctzl :: ___builtin_ctz :: ___builtin_clzll ::
+ ___builtin_clzl :: ___builtin_clz :: ___builtin_bswap64 ::
+ ___compcert_i64_umulh :: ___compcert_i64_smulh :: ___compcert_i64_sar ::
+ ___compcert_i64_shr :: ___compcert_i64_shl :: ___compcert_i64_umod ::
+ ___compcert_i64_smod :: ___compcert_i64_udiv :: ___compcert_i64_sdiv ::
+ ___compcert_i64_utof :: ___compcert_i64_stof :: ___compcert_i64_utod ::
+ ___compcert_i64_stod :: ___compcert_i64_dtou :: ___compcert_i64_dtos ::
+ ___compcert_va_composite :: ___compcert_va_float64 ::
+ ___compcert_va_int64 :: ___compcert_va_int32 :: ___builtin_va_end ::
+ ___builtin_va_copy :: ___builtin_va_arg :: ___builtin_va_start ::
+ ___builtin_membar :: ___builtin_annot_intval :: ___builtin_annot ::
+ ___builtin_memcpy_aligned :: ___builtin_fsqrt :: ___builtin_fabs ::
+ ___builtin_bswap16 :: ___builtin_bswap32 :: ___builtin_bswap ::
+ ___builtin_ais_annot :: nil).
 
 Definition prog : Clight.program := 
   mkprogram composites global_definitions public_idents _main Logic.I.
