dig/digests.v
@@ -1,179 +1,194 @@
-
-Require Import Clightdefs.
+From Coq Require Import String List ZArith.
+From compcert Require Import Coqlib Integers Floats AST Ctypes Cop Clight Clightdefs.
 Local Open Scope Z_scope.
-Definition _CRYPTO_once : ident := 166%positive.
-Definition _ERR_put_error : ident := 72%positive.
-Definition _EVP_Digest : ident := 113%positive.
-Definition _EVP_DigestFinal : ident := 107%positive.
-Definition _EVP_DigestFinal_ex : ident := 106%positive.
-Definition _EVP_DigestInit : ident := 100%positive.
-Definition _EVP_DigestInit_ex : ident := 99%positive.
-Definition _EVP_DigestUpdate : ident := 103%positive.
-Definition _EVP_MD_CTX_block_size : ident := 116%positive.
-Definition _EVP_MD_CTX_cleanup : ident := 89%positive.
-Definition _EVP_MD_CTX_copy : ident := 96%positive.
-Definition _EVP_MD_CTX_copy_ex : ident := 95%positive.
-Definition _EVP_MD_CTX_create : ident := 88%positive.
-Definition _EVP_MD_CTX_destroy : ident := 90%positive.
-Definition _EVP_MD_CTX_init : ident := 87%positive.
-Definition _EVP_MD_CTX_md : ident := 114%positive.
-Definition _EVP_MD_CTX_size : ident := 115%positive.
-Definition _EVP_MD_CTX_type : ident := 117%positive.
-Definition _EVP_MD_block_size : ident := 85%positive.
-Definition _EVP_MD_flags : ident := 83%positive.
-Definition _EVP_MD_size : ident := 84%positive.
-Definition _EVP_MD_type : ident := 82%positive.
-Definition _EVP_add_digest : ident := 118%positive.
-Definition _EVP_md4 : ident := 176%positive.
-Definition _EVP_md4_do_init : ident := 174%positive.
-Definition _EVP_md4_init : ident := 175%positive.
-Definition _EVP_md4_once : ident := 172%positive.
-Definition _EVP_md4_once_bss_get : ident := 173%positive.
-Definition _EVP_md4_storage : ident := 170%positive.
-Definition _EVP_md4_storage_bss_get : ident := 171%positive.
-Definition _EVP_md5 : ident := 186%positive.
-Definition _EVP_md5_do_init : ident := 184%positive.
-Definition _EVP_md5_init : ident := 185%positive.
-Definition _EVP_md5_once : ident := 182%positive.
-Definition _EVP_md5_once_bss_get : ident := 183%positive.
-Definition _EVP_md5_sha1 : ident := 247%positive.
-Definition _EVP_md5_sha1_do_init : ident := 245%positive.
-Definition _EVP_md5_sha1_init : ident := 246%positive.
-Definition _EVP_md5_sha1_once : ident := 243%positive.
-Definition _EVP_md5_sha1_once_bss_get : ident := 244%positive.
-Definition _EVP_md5_sha1_storage : ident := 241%positive.
-Definition _EVP_md5_sha1_storage_bss_get : ident := 242%positive.
-Definition _EVP_md5_storage : ident := 180%positive.
-Definition _EVP_md5_storage_bss_get : ident := 181%positive.
-Definition _EVP_sha1 : ident := 196%positive.
-Definition _EVP_sha1_do_init : ident := 194%positive.
-Definition _EVP_sha1_init : ident := 195%positive.
-Definition _EVP_sha1_once : ident := 192%positive.
-Definition _EVP_sha1_once_bss_get : ident := 193%positive.
-Definition _EVP_sha1_storage : ident := 190%positive.
-Definition _EVP_sha1_storage_bss_get : ident := 191%positive.
-Definition _EVP_sha224 : ident := 206%positive.
-Definition _EVP_sha224_do_init : ident := 204%positive.
-Definition _EVP_sha224_init : ident := 205%positive.
-Definition _EVP_sha224_once : ident := 202%positive.
-Definition _EVP_sha224_once_bss_get : ident := 203%positive.
-Definition _EVP_sha224_storage : ident := 200%positive.
-Definition _EVP_sha224_storage_bss_get : ident := 201%positive.
-Definition _EVP_sha256 : ident := 216%positive.
-Definition _EVP_sha256_do_init : ident := 214%positive.
-Definition _EVP_sha256_init : ident := 215%positive.
-Definition _EVP_sha256_once : ident := 212%positive.
-Definition _EVP_sha256_once_bss_get : ident := 213%positive.
-Definition _EVP_sha256_storage : ident := 210%positive.
-Definition _EVP_sha256_storage_bss_get : ident := 211%positive.
-Definition _EVP_sha384 : ident := 226%positive.
-Definition _EVP_sha384_do_init : ident := 224%positive.
-Definition _EVP_sha384_init : ident := 225%positive.
-Definition _EVP_sha384_once : ident := 222%positive.
-Definition _EVP_sha384_once_bss_get : ident := 223%positive.
-Definition _EVP_sha384_storage : ident := 220%positive.
-Definition _EVP_sha384_storage_bss_get : ident := 221%positive.
-Definition _EVP_sha512 : ident := 236%positive.
-Definition _EVP_sha512_do_init : ident := 234%positive.
-Definition _EVP_sha512_init : ident := 235%positive.
-Definition _EVP_sha512_once : ident := 232%positive.
-Definition _EVP_sha512_once_bss_get : ident := 233%positive.
-Definition _EVP_sha512_storage : ident := 230%positive.
-Definition _EVP_sha512_storage_bss_get : ident := 231%positive.
-Definition _MD4_Final : ident := 147%positive.
-Definition _MD4_Init : ident := 145%positive.
-Definition _MD4_Update : ident := 146%positive.
-Definition _MD5_Final : ident := 150%positive.
-Definition _MD5_Init : ident := 148%positive.
-Definition _MD5_Update : ident := 149%positive.
-Definition _Nh : ident := 122%positive.
-Definition _Nl : ident := 121%positive.
-Definition _OPENSSL_cleanse : ident := 74%positive.
-Definition _OPENSSL_memcpy : ident := 78%positive.
-Definition _OPENSSL_memset : ident := 80%positive.
-Definition _SHA1_Final : ident := 153%positive.
-Definition _SHA1_Init : ident := 151%positive.
-Definition _SHA1_Update : ident := 152%positive.
-Definition _SHA224_Final : ident := 156%positive.
-Definition _SHA224_Init : ident := 154%positive.
-Definition _SHA224_Update : ident := 155%positive.
-Definition _SHA256_Final : ident := 159%positive.
-Definition _SHA256_Init : ident := 157%positive.
-Definition _SHA256_Update : ident := 158%positive.
-Definition _SHA384_Final : ident := 162%positive.
-Definition _SHA384_Init : ident := 160%positive.
-Definition _SHA384_Update : ident := 161%positive.
-Definition _SHA512_Final : ident := 165%positive.
-Definition _SHA512_Init : ident := 163%positive.
-Definition _SHA512_Update : ident := 164%positive.
-Definition __2216 : ident := 133%positive.
-Definition __2217 : ident := 131%positive.
-Definition __2279 : ident := 139%positive.
-Definition __2975 : ident := 144%positive.
-Definition ___builtin_annot : ident := 21%positive.
-Definition ___builtin_annot_intval : ident := 22%positive.
-Definition ___builtin_bswap : ident := 47%positive.
-Definition ___builtin_bswap16 : ident := 50%positive.
-Definition ___builtin_bswap32 : ident := 49%positive.
-Definition ___builtin_bswap64 : ident := 48%positive.
-Definition ___builtin_clz : ident := 51%positive.
-Definition ___builtin_clzl : ident := 52%positive.
-Definition ___builtin_clzll : ident := 53%positive.
-Definition ___builtin_ctz : ident := 54%positive.
-Definition ___builtin_ctzl : ident := 55%positive.
-Definition ___builtin_ctzll : ident := 56%positive.
-Definition ___builtin_debug : ident := 69%positive.
-Definition ___builtin_fabs : ident := 19%positive.
-Definition ___builtin_fmadd : ident := 60%positive.
-Definition ___builtin_fmax : ident := 58%positive.
-Definition ___builtin_fmin : ident := 59%positive.
-Definition ___builtin_fmsub : ident := 61%positive.
-Definition ___builtin_fnmadd : ident := 62%positive.
-Definition ___builtin_fnmsub : ident := 63%positive.
-Definition ___builtin_fsqrt : ident := 57%positive.
-Definition ___builtin_membar : ident := 23%positive.
-Definition ___builtin_memcpy_aligned : ident := 20%positive.
-Definition ___builtin_nop : ident := 68%positive.
-Definition ___builtin_read16_reversed : ident := 64%positive.
-Definition ___builtin_read32_reversed : ident := 65%positive.
-Definition ___builtin_va_arg : ident := 25%positive.
-Definition ___builtin_va_copy : ident := 26%positive.
-Definition ___builtin_va_end : ident := 27%positive.
-Definition ___builtin_va_start : ident := 24%positive.
-Definition ___builtin_write16_reversed : ident := 66%positive.
-Definition ___builtin_write32_reversed : ident := 67%positive.
-Definition ___compcert_va_composite : ident := 31%positive.
-Definition ___compcert_va_float64 : ident := 30%positive.
-Definition ___compcert_va_int32 : ident := 28%positive.
-Definition ___compcert_va_int64 : ident := 29%positive.
-Definition ___i64_dtos : ident := 32%positive.
-Definition ___i64_dtou : ident := 33%positive.
-Definition ___i64_sar : ident := 44%positive.
-Definition ___i64_sdiv : ident := 38%positive.
-Definition ___i64_shl : ident := 42%positive.
-Definition ___i64_shr : ident := 43%positive.
-Definition ___i64_smod : ident := 40%positive.
-Definition ___i64_smulh : ident := 45%positive.
-Definition ___i64_stod : ident := 34%positive.
-Definition ___i64_stof : ident := 36%positive.
-Definition ___i64_udiv : ident := 39%positive.
-Definition ___i64_umod : ident := 41%positive.
-Definition ___i64_umulh : ident := 46%positive.
-Definition ___i64_utod : ident := 35%positive.
-Definition ___i64_utof : ident := 37%positive.
-Definition ___stringlit_1 : ident := 94%positive.
+
+Module Info.
+  Definition version := "3.4"%string.
+  Definition build_number := ""%string.
+  Definition build_tag := ""%string.
+  Definition arch := "x86"%string.
+  Definition model := "32sse2"%string.
+  Definition abi := "standard"%string.
+  Definition bitsize := 32.
+  Definition big_endian := false.
+  Definition source_file := "digests.c"%string.
+  Definition normalized := true.
+End Info.
+
+Definition _CRYPTO_once : ident := 167%positive.
+Definition _ERR_put_error : ident := 73%positive.
+Definition _EVP_Digest : ident := 114%positive.
+Definition _EVP_DigestFinal : ident := 108%positive.
+Definition _EVP_DigestFinal_ex : ident := 107%positive.
+Definition _EVP_DigestInit : ident := 101%positive.
+Definition _EVP_DigestInit_ex : ident := 100%positive.
+Definition _EVP_DigestUpdate : ident := 104%positive.
+Definition _EVP_MD_CTX_block_size : ident := 117%positive.
+Definition _EVP_MD_CTX_cleanup : ident := 90%positive.
+Definition _EVP_MD_CTX_copy : ident := 97%positive.
+Definition _EVP_MD_CTX_copy_ex : ident := 96%positive.
+Definition _EVP_MD_CTX_create : ident := 89%positive.
+Definition _EVP_MD_CTX_destroy : ident := 91%positive.
+Definition _EVP_MD_CTX_init : ident := 88%positive.
+Definition _EVP_MD_CTX_md : ident := 115%positive.
+Definition _EVP_MD_CTX_size : ident := 116%positive.
+Definition _EVP_MD_CTX_type : ident := 118%positive.
+Definition _EVP_MD_block_size : ident := 86%positive.
+Definition _EVP_MD_flags : ident := 84%positive.
+Definition _EVP_MD_size : ident := 85%positive.
+Definition _EVP_MD_type : ident := 83%positive.
+Definition _EVP_add_digest : ident := 119%positive.
+Definition _EVP_md4 : ident := 177%positive.
+Definition _EVP_md4_do_init : ident := 175%positive.
+Definition _EVP_md4_init : ident := 176%positive.
+Definition _EVP_md4_once : ident := 173%positive.
+Definition _EVP_md4_once_bss_get : ident := 174%positive.
+Definition _EVP_md4_storage : ident := 171%positive.
+Definition _EVP_md4_storage_bss_get : ident := 172%positive.
+Definition _EVP_md5 : ident := 187%positive.
+Definition _EVP_md5_do_init : ident := 185%positive.
+Definition _EVP_md5_init : ident := 186%positive.
+Definition _EVP_md5_once : ident := 183%positive.
+Definition _EVP_md5_once_bss_get : ident := 184%positive.
+Definition _EVP_md5_sha1 : ident := 248%positive.
+Definition _EVP_md5_sha1_do_init : ident := 246%positive.
+Definition _EVP_md5_sha1_init : ident := 247%positive.
+Definition _EVP_md5_sha1_once : ident := 244%positive.
+Definition _EVP_md5_sha1_once_bss_get : ident := 245%positive.
+Definition _EVP_md5_sha1_storage : ident := 242%positive.
+Definition _EVP_md5_sha1_storage_bss_get : ident := 243%positive.
+Definition _EVP_md5_storage : ident := 181%positive.
+Definition _EVP_md5_storage_bss_get : ident := 182%positive.
+Definition _EVP_sha1 : ident := 197%positive.
+Definition _EVP_sha1_do_init : ident := 195%positive.
+Definition _EVP_sha1_init : ident := 196%positive.
+Definition _EVP_sha1_once : ident := 193%positive.
+Definition _EVP_sha1_once_bss_get : ident := 194%positive.
+Definition _EVP_sha1_storage : ident := 191%positive.
+Definition _EVP_sha1_storage_bss_get : ident := 192%positive.
+Definition _EVP_sha224 : ident := 207%positive.
+Definition _EVP_sha224_do_init : ident := 205%positive.
+Definition _EVP_sha224_init : ident := 206%positive.
+Definition _EVP_sha224_once : ident := 203%positive.
+Definition _EVP_sha224_once_bss_get : ident := 204%positive.
+Definition _EVP_sha224_storage : ident := 201%positive.
+Definition _EVP_sha224_storage_bss_get : ident := 202%positive.
+Definition _EVP_sha256 : ident := 217%positive.
+Definition _EVP_sha256_do_init : ident := 215%positive.
+Definition _EVP_sha256_init : ident := 216%positive.
+Definition _EVP_sha256_once : ident := 213%positive.
+Definition _EVP_sha256_once_bss_get : ident := 214%positive.
+Definition _EVP_sha256_storage : ident := 211%positive.
+Definition _EVP_sha256_storage_bss_get : ident := 212%positive.
+Definition _EVP_sha384 : ident := 227%positive.
+Definition _EVP_sha384_do_init : ident := 225%positive.
+Definition _EVP_sha384_init : ident := 226%positive.
+Definition _EVP_sha384_once : ident := 223%positive.
+Definition _EVP_sha384_once_bss_get : ident := 224%positive.
+Definition _EVP_sha384_storage : ident := 221%positive.
+Definition _EVP_sha384_storage_bss_get : ident := 222%positive.
+Definition _EVP_sha512 : ident := 237%positive.
+Definition _EVP_sha512_do_init : ident := 235%positive.
+Definition _EVP_sha512_init : ident := 236%positive.
+Definition _EVP_sha512_once : ident := 233%positive.
+Definition _EVP_sha512_once_bss_get : ident := 234%positive.
+Definition _EVP_sha512_storage : ident := 231%positive.
+Definition _EVP_sha512_storage_bss_get : ident := 232%positive.
+Definition _MD4_Final : ident := 148%positive.
+Definition _MD4_Init : ident := 146%positive.
+Definition _MD4_Update : ident := 147%positive.
+Definition _MD5_Final : ident := 151%positive.
+Definition _MD5_Init : ident := 149%positive.
+Definition _MD5_Update : ident := 150%positive.
+Definition _Nh : ident := 123%positive.
+Definition _Nl : ident := 122%positive.
+Definition _OPENSSL_cleanse : ident := 75%positive.
+Definition _OPENSSL_memcpy : ident := 79%positive.
+Definition _OPENSSL_memset : ident := 81%positive.
+Definition _SHA1_Final : ident := 154%positive.
+Definition _SHA1_Init : ident := 152%positive.
+Definition _SHA1_Update : ident := 153%positive.
+Definition _SHA224_Final : ident := 157%positive.
+Definition _SHA224_Init : ident := 155%positive.
+Definition _SHA224_Update : ident := 156%positive.
+Definition _SHA256_Final : ident := 160%positive.
+Definition _SHA256_Init : ident := 158%positive.
+Definition _SHA256_Update : ident := 159%positive.
+Definition _SHA384_Final : ident := 163%positive.
+Definition _SHA384_Init : ident := 161%positive.
+Definition _SHA384_Update : ident := 162%positive.
+Definition _SHA512_Final : ident := 166%positive.
+Definition _SHA512_Init : ident := 164%positive.
+Definition _SHA512_Update : ident := 165%positive.
+Definition __2241 : ident := 134%positive.
+Definition __2242 : ident := 132%positive.
+Definition __2304 : ident := 140%positive.
+Definition __3014 : ident := 145%positive.
+Definition ___builtin_ais_annot : ident := 19%positive.
+Definition ___builtin_annot : ident := 26%positive.
+Definition ___builtin_annot_intval : ident := 27%positive.
+Definition ___builtin_bswap : ident := 20%positive.
+Definition ___builtin_bswap16 : ident := 22%positive.
+Definition ___builtin_bswap32 : ident := 21%positive.
+Definition ___builtin_bswap64 : ident := 52%positive.
+Definition ___builtin_clz : ident := 53%positive.
+Definition ___builtin_clzl : ident := 54%positive.
+Definition ___builtin_clzll : ident := 55%positive.
+Definition ___builtin_ctz : ident := 56%positive.
+Definition ___builtin_ctzl : ident := 57%positive.
+Definition ___builtin_ctzll : ident := 58%positive.
+Definition ___builtin_debug : ident := 70%positive.
+Definition ___builtin_fabs : ident := 23%positive.
+Definition ___builtin_fmadd : ident := 61%positive.
+Definition ___builtin_fmax : ident := 59%positive.
+Definition ___builtin_fmin : ident := 60%positive.
+Definition ___builtin_fmsub : ident := 62%positive.
+Definition ___builtin_fnmadd : ident := 63%positive.
+Definition ___builtin_fnmsub : ident := 64%positive.
+Definition ___builtin_fsqrt : ident := 24%positive.
+Definition ___builtin_membar : ident := 28%positive.
+Definition ___builtin_memcpy_aligned : ident := 25%positive.
+Definition ___builtin_nop : ident := 69%positive.
+Definition ___builtin_read16_reversed : ident := 65%positive.
+Definition ___builtin_read32_reversed : ident := 66%positive.
+Definition ___builtin_va_arg : ident := 30%positive.
+Definition ___builtin_va_copy : ident := 31%positive.
+Definition ___builtin_va_end : ident := 32%positive.
+Definition ___builtin_va_start : ident := 29%positive.
+Definition ___builtin_write16_reversed : ident := 67%positive.
+Definition ___builtin_write32_reversed : ident := 68%positive.
+Definition ___compcert_i64_dtos : ident := 37%positive.
+Definition ___compcert_i64_dtou : ident := 38%positive.
+Definition ___compcert_i64_sar : ident := 49%positive.
+Definition ___compcert_i64_sdiv : ident := 43%positive.
+Definition ___compcert_i64_shl : ident := 47%positive.
+Definition ___compcert_i64_shr : ident := 48%positive.
+Definition ___compcert_i64_smod : ident := 45%positive.
+Definition ___compcert_i64_smulh : ident := 50%positive.
+Definition ___compcert_i64_stod : ident := 39%positive.
+Definition ___compcert_i64_stof : ident := 41%positive.
+Definition ___compcert_i64_udiv : ident := 44%positive.
+Definition ___compcert_i64_umod : ident := 46%positive.
+Definition ___compcert_i64_umulh : ident := 51%positive.
+Definition ___compcert_i64_utod : ident := 40%positive.
+Definition ___compcert_i64_utof : ident := 42%positive.
+Definition ___compcert_va_composite : ident := 36%positive.
+Definition ___compcert_va_float64 : ident := 35%positive.
+Definition ___compcert_va_int32 : ident := 33%positive.
+Definition ___compcert_va_int64 : ident := 34%positive.
+Definition ___stringlit_1 : ident := 95%positive.
 Definition _block_size : ident := 15%positive.
-Definition _c : ident := 79%positive.
-Definition _count : ident := 108%positive.
-Definition _ctx : ident := 86%positive.
+Definition _c : ident := 80%positive.
+Definition _count : ident := 109%positive.
+Definition _ctx : ident := 87%positive.
 Definition _ctx_size : ident := 16%positive.
-Definition _d : ident := 137%positive.
-Definition _data : ident := 101%positive.
+Definition _d : ident := 138%positive.
+Definition _data : ident := 102%positive.
 Definition _digest : ident := 2%positive.
-Definition _dst : ident := 75%positive.
+Definition _dst : ident := 76%positive.
 Definition _dup : ident := 18%positive.
-Definition _engine : ident := 97%positive.
-Definition _engine_st : ident := 98%positive.
+Definition _engine : ident := 98%positive.
+Definition _engine_st : ident := 99%positive.
 Definition _env_md_ctx_st : ident := 8%positive.
 Definition _env_md_st : ident := 1%positive.
 Definition _evp_md_pctx_ops : ident := 6%positive.
@@ -181,75 +196,75 @@ Definition _evp_pkey_ctx_st : ident := 4%positive.
 Definition _final : ident := 14%positive.
 Definition _flags : ident := 11%positive.
 Definition _free : ident := 17%positive.
-Definition _h : ident := 120%positive.
-Definition _h0 : ident := 126%positive.
-Definition _h1 : ident := 127%positive.
-Definition _h2 : ident := 128%positive.
-Definition _h3 : ident := 129%positive.
-Definition _h4 : ident := 130%positive.
-Definition _impl : ident := 111%positive.
-Definition _in : ident := 92%positive.
+Definition _h : ident := 121%positive.
+Definition _h0 : ident := 127%positive.
+Definition _h1 : ident := 128%positive.
+Definition _h2 : ident := 129%positive.
+Definition _h3 : ident := 130%positive.
+Definition _h4 : ident := 131%positive.
+Definition _impl : ident := 112%positive.
+Definition _in : ident := 93%positive.
 Definition _init : ident := 12%positive.
-Definition _len : ident := 102%positive.
-Definition _main : ident := 119%positive.
-Definition _malloc : ident := 73%positive.
-Definition _md : ident := 81%positive.
-Definition _md4_final : ident := 169%positive.
-Definition _md4_init : ident := 167%positive.
-Definition _md4_state_st : ident := 124%positive.
-Definition _md4_update : ident := 168%positive.
-Definition _md5 : ident := 142%positive.
-Definition _md5_final : ident := 179%positive.
-Definition _md5_init : ident := 177%positive.
-Definition _md5_sha1_final : ident := 240%positive.
-Definition _md5_sha1_init : ident := 238%positive.
-Definition _md5_sha1_update : ident := 239%positive.
-Definition _md5_state_st : ident := 125%positive.
-Definition _md5_update : ident := 178%positive.
-Definition _md_ctx : ident := 237%positive.
+Definition _len : ident := 103%positive.
+Definition _main : ident := 120%positive.
+Definition _malloc : ident := 74%positive.
+Definition _md : ident := 82%positive.
+Definition _md4_final : ident := 170%positive.
+Definition _md4_init : ident := 168%positive.
+Definition _md4_state_st : ident := 125%positive.
+Definition _md4_update : ident := 169%positive.
+Definition _md5 : ident := 143%positive.
+Definition _md5_final : ident := 180%positive.
+Definition _md5_init : ident := 178%positive.
+Definition _md5_sha1_final : ident := 241%positive.
+Definition _md5_sha1_init : ident := 239%positive.
+Definition _md5_sha1_update : ident := 240%positive.
+Definition _md5_state_st : ident := 126%positive.
+Definition _md5_update : ident := 179%positive.
+Definition _md_ctx : ident := 238%positive.
 Definition _md_data : ident := 3%positive.
-Definition _md_len : ident := 135%positive.
-Definition _md_out : ident := 104%positive.
+Definition _md_len : ident := 136%positive.
+Definition _md_out : ident := 105%positive.
 Definition _md_size : ident := 10%positive.
-Definition _memcpy : ident := 70%positive.
-Definition _memset : ident := 71%positive.
-Definition _n : ident := 77%positive.
-Definition _num : ident := 123%positive.
-Definition _out : ident := 91%positive.
-Definition _out_md : ident := 109%positive.
-Definition _out_size : ident := 110%positive.
-Definition _p : ident := 138%positive.
+Definition _memcpy : ident := 71%positive.
+Definition _memset : ident := 72%positive.
+Definition _n : ident := 78%positive.
+Definition _num : ident := 124%positive.
+Definition _out : ident := 92%positive.
+Definition _out_md : ident := 110%positive.
+Definition _out_size : ident := 111%positive.
+Definition _p : ident := 139%positive.
 Definition _pctx : ident := 5%positive.
 Definition _pctx_ops : ident := 7%positive.
-Definition _ret : ident := 112%positive.
-Definition _sha1 : ident := 143%positive.
-Definition _sha1_final : ident := 189%positive.
-Definition _sha1_init : ident := 187%positive.
-Definition _sha1_update : ident := 188%positive.
-Definition _sha224_final : ident := 199%positive.
-Definition _sha224_init : ident := 197%positive.
-Definition _sha224_update : ident := 198%positive.
-Definition _sha256_final : ident := 209%positive.
-Definition _sha256_init : ident := 207%positive.
-Definition _sha256_state_st : ident := 136%positive.
-Definition _sha256_update : ident := 208%positive.
-Definition _sha384_final : ident := 219%positive.
-Definition _sha384_init : ident := 217%positive.
-Definition _sha384_update : ident := 218%positive.
-Definition _sha512_final : ident := 229%positive.
-Definition _sha512_init : ident := 227%positive.
-Definition _sha512_state_st : ident := 141%positive.
-Definition _sha512_update : ident := 228%positive.
-Definition _sha_state_st : ident := 134%positive.
-Definition _size : ident := 105%positive.
-Definition _src : ident := 76%positive.
-Definition _tmp_buf : ident := 93%positive.
+Definition _ret : ident := 113%positive.
+Definition _sha1 : ident := 144%positive.
+Definition _sha1_final : ident := 190%positive.
+Definition _sha1_init : ident := 188%positive.
+Definition _sha1_update : ident := 189%positive.
+Definition _sha224_final : ident := 200%positive.
+Definition _sha224_init : ident := 198%positive.
+Definition _sha224_update : ident := 199%positive.
+Definition _sha256_final : ident := 210%positive.
+Definition _sha256_init : ident := 208%positive.
+Definition _sha256_state_st : ident := 137%positive.
+Definition _sha256_update : ident := 209%positive.
+Definition _sha384_final : ident := 220%positive.
+Definition _sha384_init : ident := 218%positive.
+Definition _sha384_update : ident := 219%positive.
+Definition _sha512_final : ident := 230%positive.
+Definition _sha512_init : ident := 228%positive.
+Definition _sha512_state_st : ident := 142%positive.
+Definition _sha512_update : ident := 229%positive.
+Definition _sha_state_st : ident := 135%positive.
+Definition _size : ident := 106%positive.
+Definition _src : ident := 77%positive.
+Definition _tmp_buf : ident := 94%positive.
 Definition _type : ident := 9%positive.
-Definition _u : ident := 140%positive.
+Definition _u : ident := 141%positive.
 Definition _update : ident := 13%positive.
-Definition _t'1 : ident := 248%positive.
-Definition _t'2 : ident := 249%positive.
-Definition _t'3 : ident := 250%positive.
+Definition _t'1 : ident := 249%positive.
+Definition _t'2 : ident := 250%positive.
+Definition _t'3 : ident := 251%positive.
 
 Definition f_md4_init := {|
   fn_return := tvoid;
@@ -1803,7 +1818,7 @@ Definition f_md5_sha1_init := {|
   fn_callconv := cc_default;
   fn_params := ((_md_ctx, (tptr (Tstruct _env_md_ctx_st noattr))) :: nil);
   fn_vars := nil;
-  fn_temps := ((_ctx, (tptr (Tstruct __2975 noattr))) :: (_t'3, tint) ::
+  fn_temps := ((_ctx, (tptr (Tstruct __3014 noattr))) :: (_t'3, tint) ::
                (_t'2, tint) :: (_t'1, tint) :: nil);
   fn_body :=
 (Ssequence
@@ -1818,8 +1833,8 @@ Definition f_md5_sha1_init := {|
                         tint cc_default))
       ((Eaddrof
          (Efield
-           (Ederef (Etempvar _ctx (tptr (Tstruct __2975 noattr)))
-             (Tstruct __2975 noattr)) _md5 (Tstruct _md5_state_st noattr))
+           (Ederef (Etempvar _ctx (tptr (Tstruct __3014 noattr)))
+             (Tstruct __3014 noattr)) _md5 (Tstruct _md5_state_st noattr))
          (tptr (Tstruct _md5_state_st noattr))) :: nil))
     (Sifthenelse (Etempvar _t'1 tint)
       (Ssequence
@@ -1829,8 +1844,8 @@ Definition f_md5_sha1_init := {|
                                Tnil) tint cc_default))
           ((Eaddrof
              (Efield
-               (Ederef (Etempvar _ctx (tptr (Tstruct __2975 noattr)))
-                 (Tstruct __2975 noattr)) _sha1
+               (Ederef (Etempvar _ctx (tptr (Tstruct __3014 noattr)))
+                 (Tstruct __3014 noattr)) _sha1
                (Tstruct _sha_state_st noattr))
              (tptr (Tstruct _sha_state_st noattr))) :: nil))
         (Sset _t'2 (Ecast (Etempvar _t'3 tint) tbool)))
@@ -1843,7 +1858,7 @@ Definition f_md5_sha1_update := {|
   fn_params := ((_md_ctx, (tptr (Tstruct _env_md_ctx_st noattr))) ::
                 (_data, (tptr tvoid)) :: (_count, tuint) :: nil);
   fn_vars := nil;
-  fn_temps := ((_ctx, (tptr (Tstruct __2975 noattr))) :: (_t'3, tint) ::
+  fn_temps := ((_ctx, (tptr (Tstruct __3014 noattr))) :: (_t'3, tint) ::
                (_t'2, tint) :: (_t'1, tint) :: nil);
   fn_body :=
 (Ssequence
@@ -1859,8 +1874,8 @@ Definition f_md5_sha1_update := {|
                           cc_default))
       ((Eaddrof
          (Efield
-           (Ederef (Etempvar _ctx (tptr (Tstruct __2975 noattr)))
-             (Tstruct __2975 noattr)) _md5 (Tstruct _md5_state_st noattr))
+           (Ederef (Etempvar _ctx (tptr (Tstruct __3014 noattr)))
+             (Tstruct __3014 noattr)) _md5 (Tstruct _md5_state_st noattr))
          (tptr (Tstruct _md5_state_st noattr))) ::
        (Etempvar _data (tptr tvoid)) :: (Etempvar _count tuint) :: nil))
     (Sifthenelse (Etempvar _t'1 tint)
@@ -1872,8 +1887,8 @@ Definition f_md5_sha1_update := {|
                                tint cc_default))
           ((Eaddrof
              (Efield
-               (Ederef (Etempvar _ctx (tptr (Tstruct __2975 noattr)))
-                 (Tstruct __2975 noattr)) _sha1
+               (Ederef (Etempvar _ctx (tptr (Tstruct __3014 noattr)))
+                 (Tstruct __3014 noattr)) _sha1
                (Tstruct _sha_state_st noattr))
              (tptr (Tstruct _sha_state_st noattr))) ::
            (Etempvar _data (tptr tvoid)) :: (Etempvar _count tuint) :: nil))
@@ -1887,7 +1902,7 @@ Definition f_md5_sha1_final := {|
   fn_params := ((_md_ctx, (tptr (Tstruct _env_md_ctx_st noattr))) ::
                 (_out, (tptr tuchar)) :: nil);
   fn_vars := nil;
-  fn_temps := ((_ctx, (tptr (Tstruct __2975 noattr))) :: (_t'3, tint) ::
+  fn_temps := ((_ctx, (tptr (Tstruct __3014 noattr))) :: (_t'3, tint) ::
                (_t'2, tint) :: (_t'1, tint) :: nil);
   fn_body :=
 (Ssequence
@@ -1904,8 +1919,8 @@ Definition f_md5_sha1_final := {|
       ((Etempvar _out (tptr tuchar)) ::
        (Eaddrof
          (Efield
-           (Ederef (Etempvar _ctx (tptr (Tstruct __2975 noattr)))
-             (Tstruct __2975 noattr)) _md5 (Tstruct _md5_state_st noattr))
+           (Ederef (Etempvar _ctx (tptr (Tstruct __3014 noattr)))
+             (Tstruct __3014 noattr)) _md5 (Tstruct _md5_state_st noattr))
          (tptr (Tstruct _md5_state_st noattr))) :: nil))
     (Sifthenelse (Etempvar _t'1 tint)
       (Ssequence
@@ -1918,8 +1933,8 @@ Definition f_md5_sha1_final := {|
              (Econst_int (Int.repr 16) tint) (tptr tuchar)) ::
            (Eaddrof
              (Efield
-               (Ederef (Etempvar _ctx (tptr (Tstruct __2975 noattr)))
-                 (Tstruct __2975 noattr)) _sha1
+               (Ederef (Etempvar _ctx (tptr (Tstruct __3014 noattr)))
+                 (Tstruct __3014 noattr)) _sha1
                (Tstruct _sha_state_st noattr))
              (tptr (Tstruct _sha_state_st noattr))) :: nil))
         (Sset _t'2 (Ecast (Etempvar _t'3 tint) tbool)))
@@ -2086,7 +2101,7 @@ Definition f_EVP_md5_sha1_do_init := {|
                 (Efield
                   (Ederef (Etempvar _out (tptr (Tstruct _env_md_st noattr)))
                     (Tstruct _env_md_st noattr)) _ctx_size tuint)
-                (Esizeof (Tstruct __2975 noattr) tuint)))))))))
+                (Esizeof (Tstruct __3014 noattr) tuint)))))))))
 |}.
 
 Definition composites : list composite_definition :=
@@ -2104,27 +2119,27 @@ Definition composites : list composite_definition :=
    ((_h, (tarray tuint 4)) :: (_Nl, tuint) :: (_Nh, tuint) ::
     (_data, (tarray tuchar 64)) :: (_num, tuint) :: nil)
    noattr ::
- Composite __2217 Struct
+ Composite __2242 Struct
    ((_h0, tuint) :: (_h1, tuint) :: (_h2, tuint) :: (_h3, tuint) ::
     (_h4, tuint) :: nil)
    noattr ::
- Composite __2216 Union
-   ((_h, (tarray tuint 5)) :: (132%positive, (Tstruct __2217 noattr)) :: nil)
+ Composite __2241 Union
+   ((_h, (tarray tuint 5)) :: (133%positive, (Tstruct __2242 noattr)) :: nil)
    noattr ::
  Composite _sha_state_st Struct
-   ((132%positive, (Tunion __2216 noattr)) :: (_Nl, tuint) :: (_Nh, tuint) ::
+   ((133%positive, (Tunion __2241 noattr)) :: (_Nl, tuint) :: (_Nh, tuint) ::
     (_data, (tarray tuchar 64)) :: (_num, tuint) :: nil)
    noattr ::
  Composite _sha256_state_st Struct
    ((_h, (tarray tuint 8)) :: (_Nl, tuint) :: (_Nh, tuint) ::
     (_data, (tarray tuchar 64)) :: (_num, tuint) :: (_md_len, tuint) :: nil)
    noattr ::
- Composite __2279 Union
+ Composite __2304 Union
    ((_d, (tarray tulong 16)) :: (_p, (tarray tuchar 128)) :: nil)
    noattr ::
  Composite _sha512_state_st Struct
    ((_h, (tarray tulong 8)) :: (_Nl, tulong) :: (_Nh, tulong) ::
-    (_u, (Tunion __2279 noattr)) :: (_num, tuint) :: (_md_len, tuint) :: nil)
+    (_u, (Tunion __2304 noattr)) :: (_num, tuint) :: (_md_len, tuint) :: nil)
    noattr ::
  Composite _env_md_st Struct
    ((_type, tint) :: (_md_size, tuint) :: (_flags, tuint) ::
@@ -2149,14 +2164,36 @@ Definition composites : list composite_definition :=
      (tptr (Tfunction (Tcons (tptr (Tstruct _evp_pkey_ctx_st noattr)) Tnil)
              (tptr (Tstruct _evp_pkey_ctx_st noattr)) cc_default))) :: nil)
    noattr ::
- Composite __2975 Struct
+ Composite __3014 Struct
    ((_md5, (Tstruct _md5_state_st noattr)) ::
     (_sha1, (Tstruct _sha_state_st noattr)) :: nil)
    noattr :: nil).
 
-Definition global_definitions :=
-((___builtin_fabs,
+Definition global_definitions : list (ident * globdef fundef type) :=
+((___builtin_ais_annot,
+   Gfun(External (EF_builtin "__builtin_ais_annot"
+                   (mksignature (AST.Tint :: nil) None
+                     {|cc_vararg:=true; cc_unproto:=false; cc_structret:=false|}))
+     (Tcons (tptr tschar) Tnil) tvoid
+     {|cc_vararg:=true; cc_unproto:=false; cc_structret:=false|})) ::
+ (___builtin_bswap,
+   Gfun(External (EF_builtin "__builtin_bswap"
+                   (mksignature (AST.Tint :: nil) (Some AST.Tint) cc_default))
+     (Tcons tuint Tnil) tuint cc_default)) ::
+ (___builtin_bswap32,
+   Gfun(External (EF_builtin "__builtin_bswap32"
+                   (mksignature (AST.Tint :: nil) (Some AST.Tint) cc_default))
+     (Tcons tuint Tnil) tuint cc_default)) ::
+ (___builtin_bswap16,
+   Gfun(External (EF_builtin "__builtin_bswap16"
+                   (mksignature (AST.Tint :: nil) (Some AST.Tint) cc_default))
+     (Tcons tushort Tnil) tushort cc_default)) ::
+ (___builtin_fabs,
    Gfun(External (EF_builtin "__builtin_fabs"
+                   (mksignature (AST.Tfloat :: nil) (Some AST.Tfloat)
+                     cc_default)) (Tcons tdouble Tnil) tdouble cc_default)) ::
+ (___builtin_fsqrt,
+   Gfun(External (EF_builtin "__builtin_fsqrt"
                    (mksignature (AST.Tfloat :: nil) (Some AST.Tfloat)
                      cc_default)) (Tcons tdouble Tnil) tdouble cc_default)) ::
  (___builtin_memcpy_aligned,
@@ -2218,91 +2255,79 @@ Definition global_definitions :=
                    (mksignature (AST.Tint :: AST.Tint :: nil) (Some AST.Tint)
                      cc_default)) (Tcons (tptr tvoid) (Tcons tuint Tnil))
      (tptr tvoid) cc_default)) ::
- (___i64_dtos,
-   Gfun(External (EF_runtime "__i64_dtos"
+ (___compcert_i64_dtos,
+   Gfun(External (EF_runtime "__compcert_i64_dtos"
                    (mksignature (AST.Tfloat :: nil) (Some AST.Tlong)
                      cc_default)) (Tcons tdouble Tnil) tlong cc_default)) ::
- (___i64_dtou,
-   Gfun(External (EF_runtime "__i64_dtou"
+ (___compcert_i64_dtou,
+   Gfun(External (EF_runtime "__compcert_i64_dtou"
                    (mksignature (AST.Tfloat :: nil) (Some AST.Tlong)
                      cc_default)) (Tcons tdouble Tnil) tulong cc_default)) ::
- (___i64_stod,
-   Gfun(External (EF_runtime "__i64_stod"
+ (___compcert_i64_stod,
+   Gfun(External (EF_runtime "__compcert_i64_stod"
                    (mksignature (AST.Tlong :: nil) (Some AST.Tfloat)
                      cc_default)) (Tcons tlong Tnil) tdouble cc_default)) ::
- (___i64_utod,
-   Gfun(External (EF_runtime "__i64_utod"
+ (___compcert_i64_utod,
+   Gfun(External (EF_runtime "__compcert_i64_utod"
                    (mksignature (AST.Tlong :: nil) (Some AST.Tfloat)
                      cc_default)) (Tcons tulong Tnil) tdouble cc_default)) ::
- (___i64_stof,
-   Gfun(External (EF_runtime "__i64_stof"
+ (___compcert_i64_stof,
+   Gfun(External (EF_runtime "__compcert_i64_stof"
                    (mksignature (AST.Tlong :: nil) (Some AST.Tsingle)
                      cc_default)) (Tcons tlong Tnil) tfloat cc_default)) ::
- (___i64_utof,
-   Gfun(External (EF_runtime "__i64_utof"
+ (___compcert_i64_utof,
+   Gfun(External (EF_runtime "__compcert_i64_utof"
                    (mksignature (AST.Tlong :: nil) (Some AST.Tsingle)
                      cc_default)) (Tcons tulong Tnil) tfloat cc_default)) ::
- (___i64_sdiv,
-   Gfun(External (EF_runtime "__i64_sdiv"
+ (___compcert_i64_sdiv,
+   Gfun(External (EF_runtime "__compcert_i64_sdiv"
                    (mksignature (AST.Tlong :: AST.Tlong :: nil)
                      (Some AST.Tlong) cc_default))
      (Tcons tlong (Tcons tlong Tnil)) tlong cc_default)) ::
- (___i64_udiv,
-   Gfun(External (EF_runtime "__i64_udiv"
+ (___compcert_i64_udiv,
+   Gfun(External (EF_runtime "__compcert_i64_udiv"
                    (mksignature (AST.Tlong :: AST.Tlong :: nil)
                      (Some AST.Tlong) cc_default))
      (Tcons tulong (Tcons tulong Tnil)) tulong cc_default)) ::
- (___i64_smod,
-   Gfun(External (EF_runtime "__i64_smod"
+ (___compcert_i64_smod,
+   Gfun(External (EF_runtime "__compcert_i64_smod"
                    (mksignature (AST.Tlong :: AST.Tlong :: nil)
                      (Some AST.Tlong) cc_default))
      (Tcons tlong (Tcons tlong Tnil)) tlong cc_default)) ::
- (___i64_umod,
-   Gfun(External (EF_runtime "__i64_umod"
+ (___compcert_i64_umod,
+   Gfun(External (EF_runtime "__compcert_i64_umod"
                    (mksignature (AST.Tlong :: AST.Tlong :: nil)
                      (Some AST.Tlong) cc_default))
      (Tcons tulong (Tcons tulong Tnil)) tulong cc_default)) ::
- (___i64_shl,
-   Gfun(External (EF_runtime "__i64_shl"
+ (___compcert_i64_shl,
+   Gfun(External (EF_runtime "__compcert_i64_shl"
                    (mksignature (AST.Tlong :: AST.Tint :: nil)
                      (Some AST.Tlong) cc_default))
      (Tcons tlong (Tcons tint Tnil)) tlong cc_default)) ::
- (___i64_shr,
-   Gfun(External (EF_runtime "__i64_shr"
+ (___compcert_i64_shr,
+   Gfun(External (EF_runtime "__compcert_i64_shr"
                    (mksignature (AST.Tlong :: AST.Tint :: nil)
                      (Some AST.Tlong) cc_default))
      (Tcons tulong (Tcons tint Tnil)) tulong cc_default)) ::
- (___i64_sar,
-   Gfun(External (EF_runtime "__i64_sar"
+ (___compcert_i64_sar,
+   Gfun(External (EF_runtime "__compcert_i64_sar"
                    (mksignature (AST.Tlong :: AST.Tint :: nil)
                      (Some AST.Tlong) cc_default))
      (Tcons tlong (Tcons tint Tnil)) tlong cc_default)) ::
- (___i64_smulh,
-   Gfun(External (EF_runtime "__i64_smulh"
+ (___compcert_i64_smulh,
+   Gfun(External (EF_runtime "__compcert_i64_smulh"
                    (mksignature (AST.Tlong :: AST.Tlong :: nil)
                      (Some AST.Tlong) cc_default))
      (Tcons tlong (Tcons tlong Tnil)) tlong cc_default)) ::
- (___i64_umulh,
-   Gfun(External (EF_runtime "__i64_umulh"
+ (___compcert_i64_umulh,
+   Gfun(External (EF_runtime "__compcert_i64_umulh"
                    (mksignature (AST.Tlong :: AST.Tlong :: nil)
                      (Some AST.Tlong) cc_default))
      (Tcons tulong (Tcons tulong Tnil)) tulong cc_default)) ::
- (___builtin_bswap,
-   Gfun(External (EF_builtin "__builtin_bswap"
-                   (mksignature (AST.Tint :: nil) (Some AST.Tint) cc_default))
-     (Tcons tuint Tnil) tuint cc_default)) ::
  (___builtin_bswap64,
    Gfun(External (EF_builtin "__builtin_bswap64"
                    (mksignature (AST.Tlong :: nil) (Some AST.Tlong)
                      cc_default)) (Tcons tulong Tnil) tulong cc_default)) ::
- (___builtin_bswap32,
-   Gfun(External (EF_builtin "__builtin_bswap32"
-                   (mksignature (AST.Tint :: nil) (Some AST.Tint) cc_default))
-     (Tcons tuint Tnil) tuint cc_default)) ::
- (___builtin_bswap16,
-   Gfun(External (EF_builtin "__builtin_bswap16"
-                   (mksignature (AST.Tint :: nil) (Some AST.Tint) cc_default))
-     (Tcons tushort Tnil) tushort cc_default)) ::
  (___builtin_clz,
    Gfun(External (EF_builtin "__builtin_clz"
                    (mksignature (AST.Tint :: nil) (Some AST.Tint) cc_default))
@@ -2327,10 +2352,6 @@ Definition global_definitions :=
    Gfun(External (EF_builtin "__builtin_ctzll"
                    (mksignature (AST.Tlong :: nil) (Some AST.Tint)
                      cc_default)) (Tcons tulong Tnil) tint cc_default)) ::
- (___builtin_fsqrt,
-   Gfun(External (EF_builtin "__builtin_fsqrt"
-                   (mksignature (AST.Tfloat :: nil) (Some AST.Tfloat)
-                     cc_default)) (Tcons tdouble Tnil) tdouble cc_default)) ::
  (___builtin_fmax,
    Gfun(External (EF_builtin "__builtin_fmax"
                    (mksignature (AST.Tfloat :: AST.Tfloat :: nil)
@@ -2599,7 +2620,7 @@ Definition global_definitions :=
  (_EVP_md5_sha1, Gfun(Internal f_EVP_md5_sha1)) ::
  (_EVP_md5_sha1_do_init, Gfun(Internal f_EVP_md5_sha1_do_init)) :: nil).
 
-Definition public_idents :=
+Definition public_idents : list ident :=
 (_EVP_md5_sha1 :: _EVP_sha512 :: _EVP_sha384 :: _EVP_sha256 :: _EVP_sha224 ::
  _EVP_sha1 :: _EVP_md5 :: _EVP_md4 :: _CRYPTO_once :: _SHA512_Final ::
  _SHA512_Update :: _SHA512_Init :: _SHA384_Final :: _SHA384_Update ::
@@ -2611,17 +2632,20 @@ Definition public_idents :=
  ___builtin_write16_reversed :: ___builtin_read32_reversed ::
  ___builtin_read16_reversed :: ___builtin_fnmsub :: ___builtin_fnmadd ::
  ___builtin_fmsub :: ___builtin_fmadd :: ___builtin_fmin ::
- ___builtin_fmax :: ___builtin_fsqrt :: ___builtin_ctzll ::
- ___builtin_ctzl :: ___builtin_ctz :: ___builtin_clzll :: ___builtin_clzl ::
- ___builtin_clz :: ___builtin_bswap16 :: ___builtin_bswap32 ::
- ___builtin_bswap64 :: ___builtin_bswap :: ___i64_umulh :: ___i64_smulh ::
- ___i64_sar :: ___i64_shr :: ___i64_shl :: ___i64_umod :: ___i64_smod ::
- ___i64_udiv :: ___i64_sdiv :: ___i64_utof :: ___i64_stof :: ___i64_utod ::
- ___i64_stod :: ___i64_dtou :: ___i64_dtos :: ___compcert_va_composite ::
+ ___builtin_fmax :: ___builtin_ctzll :: ___builtin_ctzl :: ___builtin_ctz ::
+ ___builtin_clzll :: ___builtin_clzl :: ___builtin_clz ::
+ ___builtin_bswap64 :: ___compcert_i64_umulh :: ___compcert_i64_smulh ::
+ ___compcert_i64_sar :: ___compcert_i64_shr :: ___compcert_i64_shl ::
+ ___compcert_i64_umod :: ___compcert_i64_smod :: ___compcert_i64_udiv ::
+ ___compcert_i64_sdiv :: ___compcert_i64_utof :: ___compcert_i64_stof ::
+ ___compcert_i64_utod :: ___compcert_i64_stod :: ___compcert_i64_dtou ::
+ ___compcert_i64_dtos :: ___compcert_va_composite ::
  ___compcert_va_float64 :: ___compcert_va_int64 :: ___compcert_va_int32 ::
  ___builtin_va_end :: ___builtin_va_copy :: ___builtin_va_arg ::
  ___builtin_va_start :: ___builtin_membar :: ___builtin_annot_intval ::
- ___builtin_annot :: ___builtin_memcpy_aligned :: ___builtin_fabs :: nil).
+ ___builtin_annot :: ___builtin_memcpy_aligned :: ___builtin_fsqrt ::
+ ___builtin_fabs :: ___builtin_bswap16 :: ___builtin_bswap32 ::
+ ___builtin_bswap :: ___builtin_ais_annot :: nil).
 
 Definition prog : Clight.program := 
   mkprogram composites global_definitions public_idents _main Logic.I.
